$$
x^2 + 3x^1 + 2x^0 = 132\\
x = 10
$$



```
a0 = 2
a1 = 3
a2 = 1
```



```
(((1) * x + 3) * x + 2 = (x + 3) * x + 2 = x^2 + 3x + 2
(10 + 3) * 10 + 2 = 132

((0 + a2) * x + a1) * x + a0



((...(((0 * x + an) * x + an-1) * x + an-2)... + a2) * x + a1) * x + a0
```

```
a1 + b1 * i
a2 + b2 * i


(a1 + b1 * i)(a2 + b2 * i)
= a1*a2 + (a1 * b2 * i) + b1 * i * a2 - b1 * b2
= (a1 * a2 - b1 * b2) + (a1 * b2 + a2 * b1) * i

(a + b)(a - b) = a^2 - b^2

(a1 + b1 * i) / (a2 + b2 * i)
= (a1 + b1 * i)(a2 - b2 * i) / (a2 + b2 * i)(a2 - b2 * i)
= .... / (a2^2 - (b2 * i)^2)
= .... / (a2^2 + b2^2)
= (a3 + b3 * i) / k
= (a3/k) + (b3/k)*i
```


